src/program_proof/simplepb/pb_marshal_proof.v
@@ -31,7 +31,8 @@ Lemma wp_Encode (args_ptr:loc) (args:C) :
   {{{
         enc enc_sl, RET (slice_val enc_sl);
         ⌜has_encoding enc args⌝ ∗
-        is_slice enc_sl byteT 1 enc
+        is_slice enc_sl byteT 1 enc ∗
+        own args_ptr args
   }}}.
 Proof.
   iIntros (Φ) "H1 HΦ".
@@ -71,17 +72,164 @@ Proof.
   wp_load.
   iApply "HΦ".
   iFrame "Henc_sl".
-  iPureIntro.
+  iSplitL ""; first done.
+  iExists _; iFrame.
   done.
 Qed.
 
+Lemma wp_Decode enc enc_sl (args:C) :
+  {{{
+        ⌜has_encoding enc args⌝ ∗
+        is_slice enc_sl byteT 1 enc
+  }}}
+    pb.DecodeApplyArgs (slice_val enc_sl)
+  {{{
+        args_ptr, RET #args_ptr; own args_ptr args
+  }}}.
+Proof.
+  iIntros (Φ) "[%Henc Henc_sl] HΦ".
+  wp_call.
+  wp_apply (wp_ref_to).
+  { done. }
+  iIntros (enc_ptr) "Henc".
+  wp_pures.
+  wp_apply (wp_allocStruct).
+  { repeat econstructor. Transparent slice.T. unfold slice.T. repeat econstructor.
+    Opaque slice.T. }
+  iIntros (args_ptr) "Hargs".
+  iDestruct (struct_fields_split with "Hargs") as "HH".
+  iNamed "HH". simpl.
+  wp_pures.
+
+  rewrite /has_encoding in Henc.
+  rewrite Henc.
+  wp_load.
+  iDestruct (is_slice_to_small with "Henc_sl") as "Henc_sl".
+  wp_apply (wp_ReadInt with "Henc_sl").
+  iIntros (?) "Henc_sl".
+  wp_pures.
+  wp_storeField.
+  wp_store.
+
+  wp_load.
+  wp_apply (wp_ReadInt with "Henc_sl").
+  iIntros (?) "Henc_sl".
+  wp_pures.
+  wp_storeField.
+  wp_store.
+
+  wp_load.
+  wp_storeField.
+  iApply "HΦ".
+  iExists _; iFrame.
+  done.
+Qed.
 End ApplyArgs.
 
 Module SetStateArgs.
 Record C :=
 {
   epoch : u64 ;
+  state : list u8 ;
 }.
+
+Definition has_encoding (encoded:list u8) (args:C) : Prop :=
+  encoded = (u64_le args.(epoch)) ++ args.(state).
+
+Context `{!heapGS Σ}.
+
+Definition own args_ptr args : iProp Σ :=
+  ∃ state_sl,
+  "Hargs_epoch" ∷ args_ptr ↦[pb.SetStateArgs :: "Epoch"] #args.(epoch) ∗
+  "Hargs_state" ∷ args_ptr ↦[pb.SetStateArgs :: "State"] (slice_val state_sl) ∗
+  "Hargs_state_sl" ∷ is_slice_small state_sl byteT 1 args.(state)
+  .
+
+Lemma wp_Encode (args_ptr:loc) (args:C) :
+  {{{
+        own args_ptr args
+  }}}
+    pb.EncodeSetStateArgs #args_ptr
+  {{{
+        enc enc_sl, RET (slice_val enc_sl);
+        ⌜has_encoding enc args⌝ ∗
+        is_slice enc_sl byteT 1 enc ∗
+        own args_ptr args
+  }}} .
+Proof.
+  iIntros (Φ) "H1 HΦ".
+  iNamed "H1".
+  wp_call.
+  wp_loadField.
+  wp_apply (wp_slice_len).
+  wp_pures.
+  wp_apply (wp_NewSliceWithCap).
+  { apply encoding.unsigned_64_nonneg. }
+  replace (int.nat 0) with (0%nat) by word.
+  simpl.
+  iIntros (?) "Henc_sl".
+  wp_apply (wp_ref_to).
+  { done. }
+  iIntros (enc_ptr) "Henc".
+  wp_pures.
+  wp_loadField.
+  wp_load.
+  wp_apply (wp_WriteInt with "Henc_sl").
+  iIntros (?) "Henc_sl".
+  wp_store.
+  wp_loadField.
+  wp_load.
+  wp_apply (wp_WriteBytes with "[$Henc_sl $Hargs_state_sl]").
+  iIntros (?) "[Henc_sl Hargs_state_sl]".
+  wp_store.
+  wp_load.
+  iModIntro.
+  iApply "HΦ".
+  iFrame "Henc_sl".
+  iSplitL ""; first done.
+  iExists _; iFrame.
+Qed.
+
+Lemma wp_Decode enc enc_sl (args:C) :
+  {{{
+        ⌜has_encoding enc args⌝ ∗
+        is_slice enc_sl byteT 1 enc
+  }}}
+    pb.DecodeSetStateArgs (slice_val enc_sl)
+  {{{
+        args_ptr, RET #args_ptr; own args_ptr args
+  }}}.
+Proof.
+  iIntros (Φ) "[%Henc Henc_sl] HΦ".
+  wp_call.
+  wp_apply (wp_ref_to).
+  { done. }
+  iIntros (enc_ptr) "Henc".
+
+  wp_pures.
+  wp_apply (wp_allocStruct).
+  { naive_solver. }
+  iIntros (args_ptr) "Hargs".
+  iDestruct (struct_fields_split with "Hargs") as "HH".
+  iNamed "HH".
+
+  wp_pures.
+  wp_load.
+  iDestruct (is_slice_to_small with "Henc_sl") as "Henc_sl".
+  rewrite Henc.
+  wp_apply (wp_ReadInt with "Henc_sl").
+  iIntros (?) "Henc_sl".
+  wp_pures.
+  wp_storeField.
+  wp_store.
+
+  wp_load.
+  wp_storeField.
+  iModIntro.
+  iApply "HΦ".
+  iExists _; iFrame.
+Qed.
+
 End SetStateArgs.
 
 Module GetStateArgs.
@@ -89,6 +237,78 @@ Record C :=
 {
   epoch : u64 ;
 }.
+
+Definition has_encoding (encoded:list u8) (args:C) : Prop :=
+  encoded = (u64_le args.(epoch)).
+
+Context `{!heapGS Σ}.
+
+Definition own args_ptr args : iProp Σ :=
+  "Hargs_epoch" ∷ args_ptr ↦[pb.GetStateArgs :: "Epoch"] #args.(epoch)
+  .
+
+Lemma wp_Encode (args_ptr:loc) (args:C) :
+  {{{
+        own args_ptr args
+  }}}
+    pb.EncodeGetStateArgs #args_ptr
+  {{{
+        enc enc_sl, RET (slice_val enc_sl);
+        ⌜has_encoding enc args⌝ ∗
+        is_slice enc_sl byteT 1 enc
+  }}}.
+Proof.
+  iIntros (?) "H1 HΦ".
+  iNamed "H1".
+  wp_call.
+  wp_apply (wp_NewSliceWithCap).
+  { done. }
+  iIntros (?) "Henc_sl".
+  wp_apply (wp_ref_to).
+  { done. }
+  iIntros (enc_ptr) "Henc".
+  wp_pures.
+  wp_loadField.
+  wp_load.
+  wp_apply (wp_WriteInt with "Henc_sl").
+  iIntros (?) "Henc_sl".
+  wp_store.
+  wp_load.
+  iApply "HΦ".
+  iFrame.
+  done.
+Qed.
+
+Lemma wp_Decode enc enc_sl (args:C) :
+  {{{
+        ⌜has_encoding enc args⌝ ∗
+        is_slice enc_sl byteT 1 enc
+  }}}
+    pb.DecodeGetStateArgs (slice_val enc_sl)
+  {{{
+        args_ptr, RET #args_ptr; own args_ptr args
+  }}}.
+Proof.
+  iIntros (Φ) "[%Henc Henc_sl] HΦ".
+  wp_call.
+  wp_apply (wp_allocStruct).
+  { naive_solver. }
+  iIntros (args_ptr) "Hargs".
+  wp_pures.
+  iDestruct (is_slice_to_small with "Henc_sl") as "Henc_sl".
+  rewrite Henc.
+  wp_apply (wp_ReadInt with "Henc_sl").
+  iIntros (?) "Henc_sl".
+  wp_pures.
+  iDestruct (struct_fields_split with "Hargs") as "HH".
+  iNamed "HH".
+  wp_storeField.
+  wp_pures.
+  iModIntro.
+  iApply "HΦ".
+  iFrame.
+Qed.
+
 End GetStateArgs.
 
 Module GetStateReply.
@@ -97,6 +317,100 @@ Record C :=
   err : u64 ;
   state : list u8 ;
 }.
+
+Definition has_encoding (encoded:list u8) (reply:C) : Prop :=
+  encoded = (u64_le reply.(err)) ++ reply.(state).
+
+Context `{!heapGS Σ}.
+
+Definition own reply_ptr reply : iProp Σ :=
+  ∃ state_sl,
+  "Hreply_epoch" ∷ reply_ptr ↦[pb.GetStateReply :: "Err"] #reply.(err) ∗
+  "Hreply_state" ∷ reply_ptr ↦[pb.GetStateReply :: "State"] (slice_val state_sl) ∗
+  "Hreply_state_sl" ∷ is_slice_small state_sl byteT 1 reply.(state)
+  .
+
+Lemma wp_Encode (reply_ptr:loc) (reply:C) :
+  {{{
+        own reply_ptr reply
+  }}}
+    pb.EncodeGetStateReply #reply_ptr
+  {{{
+        enc enc_sl, RET (slice_val enc_sl);
+        ⌜has_encoding enc reply⌝ ∗
+        is_slice enc_sl byteT 1 enc
+  }}}.
+Proof.
+  iIntros (?) "H1 HΦ".
+  iNamed "H1".
+  wp_call.
+  wp_loadField.
+  wp_apply (wp_slice_len).
+  wp_pures.
+  wp_apply (wp_NewSliceWithCap).
+  { apply encoding.unsigned_64_nonneg. }
+  replace (int.nat 0) with (0%nat) by word.
+  simpl.
+  iIntros (?) "Henc_sl".
+  wp_apply (wp_ref_to).
+  { done. }
+  iIntros (enc_ptr) "Henc".
+  wp_pures.
+  wp_loadField.
+  wp_load.
+  wp_apply (wp_WriteInt with "Henc_sl").
+  iIntros (?) "Henc_sl".
+  wp_store.
+  wp_loadField.
+  wp_load.
+  wp_apply (wp_WriteBytes with "[$Henc_sl $Hreply_state_sl]").
+  iIntros (?) "[Henc_sl Hreply_state_sl]".
+  wp_store.
+  wp_load.
+  iModIntro.
+  iApply "HΦ".
+  iFrame.
+  done.
+Qed.
+
+Lemma wp_Decode enc enc_sl (reply:C) :
+  {{{
+        ⌜has_encoding enc reply⌝ ∗
+        is_slice enc_sl byteT 1 enc
+  }}}
+    pb.DecodeGetStateReply (slice_val enc_sl)
+  {{{
+        reply_ptr, RET #reply_ptr; own reply_ptr reply
+  }}}.
+Proof.
+  iIntros (Φ) "[%Henc Henc_sl] HΦ".
+  wp_call.
+  wp_apply (wp_ref_to).
+  { done. }
+  iIntros (enc_ptr) "Henc".
+  wp_apply (wp_allocStruct).
+  { naive_solver. }
+  iIntros (args_ptr) "Hargs".
+  iDestruct (struct_fields_split with "Hargs") as "HH".
+  iNamed "HH".
+  wp_pures.
+  iDestruct (is_slice_to_small with "Henc_sl") as "Henc_sl".
+  rewrite Henc.
+  wp_load.
+  wp_apply (wp_ReadInt with "Henc_sl").
+  iIntros (?) "Henc_sl".
+  wp_pures.
+  wp_storeField.
+  wp_store.
+
+  wp_load.
+  wp_storeField.
+
+  iModIntro.
+  iApply "HΦ".
+  iExists _; iFrame.
+Qed.
+
 End GetStateReply.
 
 Module BecomePrimaryArgs.
@@ -105,6 +419,83 @@ Record C :=
   epoch : u64 ;
   replicas : list chan ;
 }.
+
+Definition has_encoding (encoded:list u8) (args:C) : Prop :=
+  encoded = (u64_le args.(epoch)) ++ (u64_le (length args.(replicas))) ++ (flat_map u64_le args.(replicas)).
+
+Context `{!heapGS Σ}.
+
+Definition own args_ptr args : iProp Σ :=
+  ∃ replicas_sl,
+  "Hargs_epoch" ∷ args_ptr ↦[pb.BecomePrimaryArgs :: "Epoch"] #args.(epoch) ∗
+  "Hargs_replicas" ∷ args_ptr ↦[pb.BecomePrimaryArgs :: "Replicas"] (slice_val replicas_sl) ∗
+  "Hargs_replicas_sl" ∷ is_slice_small replicas_sl uint64T 1 args.(replicas)
+  .
+
+Lemma wp_Encode (args_ptr:loc) (args:C) :
+  {{{
+        own args_ptr args
+  }}}
+    pb.EncodeBecomePrimaryArgs #args_ptr
+  {{{
+        enc enc_sl, RET (slice_val enc_sl);
+        ⌜has_encoding enc args⌝ ∗
+        is_slice enc_sl byteT 1 enc
+  }}}.
+Proof.
+  iIntros (?) "H1 HΦ".
+  iNamed "H1".
+  wp_call.
+  wp_loadField.
+  wp_apply (wp_slice_len).
+  wp_pures.
+  wp_apply (wp_NewSliceWithCap).
+  { apply encoding.unsigned_64_nonneg. }
+  replace (int.nat 0) with (0%nat) by word.
+  simpl.
+  iIntros (?) "Henc_sl".
+  wp_apply (wp_ref_to).
+  { done. }
+  iIntros (enc_ptr) "Henc".
+  wp_pures.
+  wp_loadField.
+  wp_load.
+  wp_apply (wp_WriteInt with "Henc_sl").
+  iIntros (?) "Henc_sl".
+  wp_store.
+  wp_loadField.
+  wp_apply (wp_slice_len).
+  iDestruct (is_slice_small_sz with "Hargs_replicas_sl") as %Hsz.
+  wp_load.
+  wp_apply (wp_WriteInt with "Henc_sl").
+  iIntros (?) "Henc_sl".
+  wp_store.
+  replace (replicas_sl.(Slice.sz)) with (U64 (length args.(replicas))) by word.
+
+  wp_loadField.
+  (*
+  wp_apply (wp_forSlice
+              (λ j,
+                ∃ enc_sl (replicas_so_far:list chan),
+  "%Hreplicas" ∷ True ∗
+  "Henc" ∷ enc_ptr ↦[slice.T byteT] (slice_val enc_sl) ∗
+  "Henc_sl" ∷ is_slice enc_sl byteT 1 (([] ++ u64_le args.(epoch)) ++ u64_le (length args.(replicas)) ++ (flat_map u64_le replicas_so_far))
+              )%I
+              with "[] [] []"
+           ). *)
+Admitted.
+
+Lemma wp_Decode enc enc_sl (args:C) :
+  {{{
+        ⌜has_encoding enc args⌝ ∗
+        is_slice enc_sl byteT 1 enc
+  }}}
+    pb.DecodeBecomePrimaryArgs (slice_val enc_sl)
+  {{{
+        args_ptr, RET #args_ptr; own args_ptr args
+  }}}.
+Admitted.
+
 End BecomePrimaryArgs.
 
 Section pb_marshal.
